refactor: introduce SSA typeclass to (incrementally) replace axioms

EffectSSA/ProofSketch/InstSeq.lean
@@ -1,8 +1,8 @@
 module
 
-public import EffectSSA.ProofSketch.Inst
 public import EffectSSA.ProofSketch.VarSet
 public import EffectSSA.ProofSketch.Effect
+public import EffectSSA.ProofSketch.Assumptions
 
 /-!
 # Instruction Sequence
@@ -11,7 +11,7 @@ namespace EffectSSA.ProofSketch
 open VarSet
 open ITree
 
-public abbrev InstSeq := List Inst
+public abbrev InstSeq ι := List ι
 
 
 /-!
@@ -22,7 +22,7 @@ We then also include custom induction & cases principle for the same purpose.
 -/
 section Cons
 
-@[grind, match_pattern] public abbrev InstSeq.cons : Inst → InstSeq → InstSeq :=
+@[grind, match_pattern] public abbrev InstSeq.cons : ι → InstSeq ι → InstSeq ι :=
   (· :: ·)
 
 scoped infixl:67 " ;> " => InstSeq.cons
@@ -30,15 +30,15 @@ scoped infixl:67 " ;> " => InstSeq.cons
 namespace InstSeq
 
 @[induction_eliminator, elab_as_elim]
-public noncomputable def rec {motive : InstSeq → Sort u} :
+public noncomputable def rec {motive : InstSeq ι → Sort u} :
     (nil : motive []) →
-    (cons : (head : Inst) → (tail : InstSeq) → motive tail → motive (head ;> tail)) →
+    (cons : (head : ι) → (tail : InstSeq ι) → motive tail → motive (head ;> tail)) →
     ∀ is, motive is := List.rec
 
 @[cases_eliminator, elab_as_elim]
-public noncomputable def cases {motive : InstSeq → Sort u}
+public noncomputable def cases {motive : InstSeq ι → Sort u}
     (nil : motive [])
-    (cons : (head : Inst) → (tail : InstSeq) → motive (head ;> tail)) :
+    (cons : (head : ι) → (tail : InstSeq ι) → motive (head ;> tail)) :
     ∀ is, motive is :=
   (List.casesOn · nil cons)
 
@@ -47,6 +47,7 @@ end Cons
 
 namespace InstSeq
 
+variable {ι : Type} {σ : Type} [SSA ι σ]
 variable {ε : Type} {κ : ε → Type} [Effect ε κ]
 
 /-!
@@ -57,7 +58,7 @@ variable {ε : Type} {κ : ε → Type} [Effect ε κ]
 Denote an `InstSeq` into an ITree with `InstEff`s, i.e,
 where each instruction has a unique effect associated with it.
 -/
-public def denote : (is : InstSeq) → ITree InstEff Unit
+public def denote : (is : InstSeq Inst) → ITree InstEff Unit
   | i :: is => Effect.trigger InstEff i *> denote is
   | [] => .ret ()
 
@@ -65,14 +66,15 @@ public def denote : (is : InstSeq) → ITree InstEff Unit
 ## Variables
 -/
 noncomputable section Vars
+open SSA (args results)
 
 @[grind]
-def argsResults : InstSeq → VarSet × VarSet := go ∅ ∅
+def argsResults : InstSeq ι → VarSet × VarSet := go ∅ ∅
 where go (A R : VarSet)
   | [] => (A, R)
   | i ;> is =>
-    let A := A ∪ (i.args - R)
-    let R := R ∪ i.results
+    let A := A ∪ (args i - R)
+    let R := R ∪ results i
     go A R is
 
 /--
@@ -81,15 +83,15 @@ where go (A R : VarSet)
 Note: "free" means that any argument of an instruction `i ∈ is` that is also the
 result of any preceding instructions are *not* included in `is.args`.
 -/
-public def args (is : InstSeq) : VarSet :=
+public def args (is : InstSeq ι) : VarSet :=
   is.argsResults.1
 
 /-- `is.results` is the set of all results of sequence `is`. -/
-public def results (is : InstSeq) : VarSet :=
+public def results (is : InstSeq ι) : VarSet :=
   is.argsResults.2
 
 section Lemmas
-variable {i : Inst} {is : InstSeq}
+variable {i : ι} {is : InstSeq ι}
 attribute [local grind] results args argsResults argsResults.go
 
 @[grind =] theorem argsResults_go_fst (A R : VarSet) :
@@ -99,9 +101,9 @@ attribute [local grind] results args argsResults argsResults.go
   by simp [args, argsResults]; grind
   induction is generalizing A R <;> grind
 
-@[simp, grind =] public theorem args_nil : args [] = ∅ := by rfl
+@[simp, grind =] public theorem args_nil : args ([] : InstSeq ι) = ∅ := by rfl
 @[simp, grind =] public theorem args_cons :
-    args (i ;> is) = i.args ∪ (args is - i.results) := by
+    args (i ;> is) = SSA.args i ∪ (args is - SSA.results i) := by
   show (argsResults.go ..).fst = _; grind
 
 @[grind =] theorem argsResults_go_snd : (argsResults.go A R is).2 = R ∪ is.results := by
@@ -110,22 +112,22 @@ attribute [local grind] results args argsResults argsResults.go
   by simp [results, argsResults]; grind
   induction is generalizing A R <;> grind
 
-@[simp, grind =] public theorem results_nil  : results [] = ∅ := by rfl
-@[simp, grind =] public theorem results_cons : results (i ;> is) = i.results ∪ is.results := by
+@[simp, grind =] public theorem results_nil  : results ([] : InstSeq ι) = ∅ := by rfl
+@[simp, grind =] public theorem results_cons : results (i ;> is) = SSA.results i ∪ is.results := by
   show (argsResults.go ..).snd = _; grind
 
-@[simp, grind =] public theorem results_append {xs ys : InstSeq} :
+@[simp, grind =] public theorem results_append {xs ys : InstSeq ι} :
     results (xs ++ ys) = xs.results ∪ ys.results := by
   induction xs <;> grind
 
-@[grind =] public theorem mem_results_iff : x ∈ is.results ↔ ∃ i ∈ is, x ∈ i.results := by
+@[grind =] public theorem mem_results_iff : x ∈ is.results ↔ ∃ i ∈ is, x ∈ SSA.results i := by
   induction is <;> grind
 
-@[grind →] public theorem mem_results_of_mem_inst {x : VarId} (hi : i ∈ is) (hx : x ∈ i.results) :
+@[grind →] public theorem mem_results_of_mem_inst {x : VarId} (hi : i ∈ is) (hx : x ∈ SSA.results i) :
     x ∈ is.results := by
   grind
 
-@[grind →] public theorem results_subset_of_mem (h : i ∈ is) : i.results ⊆ is.results := by
+@[grind →] public theorem results_subset_of_mem (h : i ∈ is) : SSA.results i ⊆ is.results := by
   grind
 
 /--
@@ -135,7 +137,7 @@ free (thus in `is.args`), or might refer to the result of an earlier instruction
 the latter we over-approximate by the results of all instructions (`is.results`)
 -/
 @[grind →] public theorem args_subset_of_mem (h : i ∈ is) :
-    i.args ⊆ is.args ∪ is.results := by
+    SSA.args i ⊆ is.args ∪ is.results := by
   induction is <;> grind
 
 end Lemmas
@@ -146,20 +148,20 @@ end Lemmas
 `is.getDef? v` returns an instruction `i ∈ is` s.t. `v ∈ i.results`,
 or `none` if no such instruction exists
 -/
-public noncomputable def getDef? (v : VarId) : (is : InstSeq) → Option { i // i ∈ is ∧ v ∈ is.results }
+public noncomputable def getDef? (v : VarId) : (is : InstSeq ι) → Option { i // i ∈ is ∧ v ∈ is.results }
   | [] => none
   | i ;> is =>
       open Classical in
-      if hi : v ∈ i.results then
+      if hi : v ∈ SSA.results i then
         some ⟨i, by grind⟩
       else
         (getDef? v is).map (fun ⟨i, hi⟩ => ⟨i, by grind⟩)
 
 /-- `is.UsesAt y x` is true when `y` is a (transitive) dependency of `x`. -/
 @[grind cases]
-public inductive UsesAt (is : InstSeq) (y : VarId) : VarId → Prop
-  | arg  : i ∈ is → x ∈ i.results → y ∈ i.args → UsesAt is y x
-  | trans : i ∈ is → x ∈ i.results → z ∈ i.args → UsesAt is y z → UsesAt is y x
+public inductive UsesAt (is : InstSeq ι) (y : VarId) : VarId → Prop
+  | arg  : i ∈ is → x ∈ SSA.results i → y ∈ SSA.args i → UsesAt is y x
+  | trans : i ∈ is → x ∈ SSA.results i → z ∈ SSA.args i → UsesAt is y z → UsesAt is y x
 
 /--
 `is.usesAt v` is the set of all transitive arguments that are used to compute
@@ -171,17 +173,17 @@ union of `i.args` with the recursive set `{ is.usesAt y | y ∈ i.args }`.
 If no instruction of `is` defines the variable `v` as a result,
 then `is.usesAt v` is the empty set.
 -/
-public def usesAt (x : VarId) (is : InstSeq) : VarSet :=
+public def usesAt (x : VarId) (is : InstSeq ι) : VarSet :=
   { y | is.UsesAt y x }
 
 section Lemmas
-variable {is : InstSeq}
+variable {is : InstSeq ι}
 
 @[simp, grind =] public theorem mem_usesAt : y ∈ is.usesAt x ↔ is.UsesAt y x := by
   simp [usesAt]
 
 public theorem mem_usesAt' :
-    y ∈ is.usesAt x ↔ ∃ i ∈ is, x ∈ i.results ∧ (y ∈ i.args ∨ ∃ z ∈ i.args, y ∈ is.usesAt z) := by
+    y ∈ is.usesAt x ↔ ∃ i ∈ is, x ∈ SSA.results i ∧ (y ∈ SSA.args i ∨ ∃ z ∈ SSA.args i, y ∈ is.usesAt z) := by
   constructor
   · grind
   · simp only [mem_usesAt, forall_exists_index, and_imp]
@@ -189,8 +191,8 @@ public theorem mem_usesAt' :
     · apply UsesAt.arg hi hxi hy
     · apply UsesAt.trans hi hxi hzi hyz
 
-@[simp, grind .] public theorem not_usesAt_nil : ¬(UsesAt [] y x) := by grind
-@[simp, grind =] public theorem usesAt_nil_eq : usesAt x [] = ∅ := by grind
+@[simp, grind .] public theorem not_usesAt_nil : ¬(UsesAt ([] : InstSeq ι) y x) := by grind
+@[simp, grind =] public theorem usesAt_nil_eq : usesAt x ([] : InstSeq ι) = ∅ := by grind
 
 @[simp, grind =>]
 public theorem usesAt_eq_of_not_mem_results {x : VarId} (h : x ∉ is.results) :
@@ -214,7 +216,7 @@ index into the sequence), as well as a way to index into the sequence with
 a PC.
 -/
 public section PC
-variable {is js : InstSeq}
+variable {is js : InstSeq ι}
 
 /--
 `is.PC` is the type of program counters of the sequence `is`.
@@ -222,7 +224,7 @@ variable {is js : InstSeq}
 Each program counter `pc : is.PC` uniquely identifies a location of the program.
 -/
 @[grind cases, grind]
-structure PC (is : InstSeq) : Type where
+structure PC (is : InstSeq ι) : Type where
   idx : Nat
   isLt : idx < is.length := by grind
 
@@ -231,7 +233,7 @@ structure PC (is : InstSeq) : Type where
   isLt := i.isLt
 
 /-- Get the instruction at the specified location. -/
-@[expose] def PC.get (pc : is.PC) : Inst := is[pc.idx]'pc.isLt
+@[expose] def PC.get (pc : is.PC) : ι := is[pc.idx]'pc.isLt
 
 section Lemmas
 
@@ -258,15 +260,15 @@ namespace PC
 
 /-! cases principle -/
 
-@[grind] def zero {i is} : PC (i ;> is) where idx := 0
-@[grind] def succ {i is} (p : PC is) : PC (i ;> is) where idx := p.idx + 1
+@[grind] def zero {i : ι} {is : InstSeq ι} : PC (i ;> is) where idx := 0
+@[grind] def succ {i : ι} {is : InstSeq ι} (p : PC is) : PC (i ;> is) where idx := p.idx + 1
 
-@[grind =, simp] theorem get_zero : (@zero i is).get = i := by rfl
+@[grind =, simp] theorem get_zero : (@zero _ i is).get = i := by rfl
 @[grind =, simp] theorem get_succ (p : PC is) :
-    (@p.succ i _).get (is := no_index _) = p.get := by rfl
+    (@p.succ _ i _).get (is := no_index _) = p.get := by rfl
 
 @[grind =, simp] theorem succ_eq_succ_iff {p q : is.PC} :
-    (@p.succ i is) = q.succ ↔ p = q := by grind
+    (@p.succ _ i is) = q.succ ↔ p = q := by grind
 
 @[cases_eliminator, elab_as_elim]
 def consCases {motive : PC (i ;> is) → Prop}
@@ -278,27 +280,27 @@ def consCases {motive : PC (i ;> is) → Prop}
   case succ n => apply cast ?_ (succ ⟨n, by grind⟩); grind
 
 /-! append -/
-variable {is js : InstSeq}
+variable {is js : InstSeq ι}
 
 def appendLeft (p : PC is) : PC (is ++ js) where idx := p.idx
 def appendRight (p : PC js) : PC (is ++ js) where idx := p.idx + is.length
 
 @[grind =, simp] theorem idx_appendLeft :
-    (@appendLeft is js p).idx = p.idx := by rfl
+    (@appendLeft _ is js p).idx = p.idx := by rfl
 
 @[grind =, simp] theorem idx_appendRight :
-    (@appendRight is js p).idx = p.idx + is.length := by rfl
+    (@appendRight _ is js p).idx = p.idx + is.length := by rfl
 
 @[grind =, simp] theorem get_appendLeft {p : PC is} :
-    (@appendLeft is js p).get = p.get := by grind [get]
+    (@appendLeft _ is js p).get = p.get := by grind [get]
 
 @[grind =, simp] theorem get_appendRight {p : PC js} :
-    (@appendRight is js p).get = p.get := by grind [get]
+    (@appendRight _ is js p).get = p.get := by grind [get]
 
 @[grind =, simp] theorem appendLeft_eq_appendLeft_iff (p q : PC is) :
-    (@p.appendLeft is js) = q.appendLeft ↔ p = q := by grind [appendLeft]
+    (@p.appendLeft _ is js) = q.appendLeft ↔ p = q := by grind [appendLeft]
 @[grind =, simp] theorem appendRight_eq_appendRight_iff (p q : PC js) :
-    (@p.appendRight is js) = q.appendRight ↔ p = q := by grind [appendRight]
+    (@p.appendRight _ is js) = q.appendRight ↔ p = q := by grind [appendRight]
 @[grind ., simp] theorem appendLeft_neq_appendRight (p : PC is) (q : PC js) :
     p.appendLeft ≠ q.appendRight := by grind [appendLeft, appendRight]
 
@@ -322,7 +324,7 @@ end Lemmas
 
 /-! Map PCs of `is` or `js` into `is ++ js`. -/
 section OfAppend
-variable {is js : InstSeq}
+variable {is js : InstSeq ι}
 
 public def PC.ofAppendLeft : is.PC → (is ++ js).PC
   | ⟨idx, isLt⟩ => ⟨idx, by grind⟩
@@ -333,11 +335,11 @@ public def PC.ofAppendRight : js.PC → (is ++ js).PC
 section AppendLemmas
 
 @[simp, grind =] public theorem get_ofAppendLeft :
-    (@PC.ofAppendLeft is js p).get = p.get := by
+    (@PC.ofAppendLeft _ is js p).get = p.get := by
   grind [PC.get, PC.ofAppendLeft]
 
 @[simp, grind =] public theorem get_ofAppendRight :
-    (@PC.ofAppendRight is js p).get = p.get := by
+    (@PC.ofAppendRight _ is js p).get = p.get := by
   grind [PC.get, PC.ofAppendRight]
 
 end AppendLemmas
@@ -353,13 +355,13 @@ program in another.
 -/
 public section Embed
 
-structure EmbedIn (is js : InstSeq) where
+structure EmbedIn (is js : InstSeq ι) where
   map : is.PC → js.PC
   get_map : ∀ i, (map i).get = i.get
-  inj : ∀ i j : is.PC, i ≠ j → i.get.results ≠ ∅ → j.get.results ≠ ∅ → map i ≠ map j
+  inj : ∀ i j : is.PC, i ≠ j → SSA.results i.get ≠ ∅ → SSA.results j.get ≠ ∅ → map i ≠ map j
 
 -- `f : is.EmbedIn js` can be used a function
-instance {is js : InstSeq} : CoeFun (is.EmbedIn js) (fun _ => is.PC → js.PC) where
+instance {is js : InstSeq ι} : CoeFun (is.EmbedIn js) (fun _ => is.PC → js.PC) where
   coe f := f.map
 
 section Lemmas
@@ -391,10 +393,10 @@ public section WellFormed
 `is.NoShadowing` holds if no two instructions in `is` define the same
 resulting variable.
 -/
-inductive NoShadowing : InstSeq → Prop
+inductive NoShadowing : InstSeq ι → Prop
   | nil : NoShadowing []
-  | cons {i : Inst} {is : InstSeq} :
-      i.results.Disjoint is.results → NoShadowing is
+  | cons {i : ι} {is : InstSeq ι} :
+      (SSA.results i).Disjoint is.results → NoShadowing is
       → NoShadowing (i ;> is)
 
 /--
@@ -405,13 +407,13 @@ A sequence `is` is well-formed, w.r.t. free variables `Γ`, when
 * `Γ` does not contain any result of `is`.
 -/
 @[grind, grind cases]
-structure WellFormed (Γ : VarSet) (is : InstSeq)  where
+structure WellFormed (Γ : VarSet) (is : InstSeq ι) where
   noShadowing : is.NoShadowing
   args : is.args ⊆ Γ
   results : is.results.Disjoint Γ
 
 section Lemmas
-variable {is js : InstSeq}
+variable {is js : InstSeq ι}
 
 /-! ### Grind Annotations -/
 section Grind
@@ -426,18 +428,18 @@ end Grind
 section Basic
 attribute [local grind] WellFormed NoShadowing
 
-@[grind ., simp] theorem noShadowing_nil : NoShadowing [] := by grind
+@[grind ., simp] theorem noShadowing_nil : NoShadowing ([] : InstSeq ι) := by grind
 @[grind =, simp] theorem noShadowing_cons :
-    NoShadowing (i ;> is) ↔ i.results.Disjoint is.results ∧ NoShadowing is := by grind
+    NoShadowing (i ;> is) ↔ (SSA.results i).Disjoint is.results ∧ NoShadowing is := by grind
 
 @[grind =, simp] theorem noShadowing_append :
     NoShadowing (is ++ js) ↔ is.results.Disjoint js.results ∧ is.NoShadowing ∧ js.NoShadowing := by
   induction is <;> grind
 
-@[grind ., simp] theorem wellFormed_nil : WellFormed Γ [] := by grind
+@[grind ., simp] theorem wellFormed_nil : WellFormed Γ ([] : InstSeq ι) := by grind
 @[grind =, simp] theorem wellFormed_cons :
     WellFormed Γ (i ;> is) ↔
-      i.args ⊆ Γ ∧ Γ.Disjoint i.results ∧ is.WellFormed (i.results ∪ Γ) := by
+      SSA.args i ⊆ Γ ∧ Γ.Disjoint (SSA.results i) ∧ is.WellFormed (SSA.results i ∪ Γ) := by
   constructor
   · rintro ⟨⟩
     and_intros
@@ -462,11 +464,11 @@ section PC
 
 theorem noShadowing_iff :
     is.NoShadowing ↔ ∀ (i j : is.PC), i ≠ j →
-      i.get.results.Disjoint j.get.results := by
+      (SSA.results i.get).Disjoint (SSA.results j.get) := by
   induction is
   case nil => grind
   case cons i is ih =>
-    change InstSeq at is
+    change InstSeq ι at is
     simp only [noShadowing_cons, ne_eq]
     constructor
     · rintro ⟨hdj, hns⟩
@@ -474,11 +476,11 @@ theorem noShadowing_iff :
       cases j <;> cases k <;> grind
     · intro h
       and_intros
-      · suffices ∀ j ∈ is, i.results.Disjoint j.results by grind
-        suffices ∀ j : is.PC, i.results.Disjoint j.get.results by grind
+      · suffices ∀ j ∈ is, (SSA.results i).Disjoint (SSA.results j) by grind
+        suffices ∀ j : is.PC, (SSA.results i).Disjoint (SSA.results j.get) by grind
         intro j
         simpa using h .zero j.succ (by grind)
-      · suffices ∀ (i j : is.PC), i ≠ j → i.get.results.Disjoint j.get.results by grind
+      · suffices ∀ (i j : is.PC), i ≠ j → (SSA.results i.get).Disjoint (SSA.results j.get) by grind
         intro j k hjk
         simpa using h j.succ k.succ (by grind)
 
@@ -489,15 +491,15 @@ section ResultLemmas
 
 @[grind <=]
 theorem results_disjoint_of_mem_of_noShadowing (hi : i ∈ is) (hj : j ∈ is) (wf : is.NoShadowing) :
-    i ≠ j → i.results.Disjoint j.results := by
+    i ≠ j → (SSA.results i).Disjoint (SSA.results j) := by
   induction is <;> grind
 
-theorem eq_of_not_disjoint_results_of_noShadowing {i j : Inst}
+theorem eq_of_not_disjoint_results_of_noShadowing {i j : ι}
     (hi : i ∈ is) (hj : j ∈ is) (wf : is.NoShadowing) :
-    ¬(i.results.Disjoint j.results) → i = j := by
+    ¬((SSA.results i).Disjoint (SSA.results j)) → i = j := by
   induction is <;> grind
 grind_pattern eq_of_not_disjoint_results_of_noShadowing =>
-  i.results.Disjoint j.results, i ∈ is, j ∈ is, is.NoShadowing
+  (SSA.results i).Disjoint (SSA.results j), i ∈ is, j ∈ is, is.NoShadowing
   -- ^^ TODO: this pattern seems overly specific, maybe I could drop the Disjoint pattern
 
 end ResultLemmas
