EffectSSA/ProofSketch/Assumptions.lean
@@ -1,0 +1,11 @@
+module
+
+public import EffectSSA.ProofSketch.VarSet
+public import EffectSSA.ProofSketch.Denote
+
+namespace EffectSSA.ProofSketch
+
+public class SSA (ι : Type) (σ : outParam Type) : Type where
+  [decidableEq : DecidableEq ι]
+  args : ι → VarSet
+  results : ι → VarSet
